- Alle reglene her vil bruke $x$ som variabelen vi deriverer mot, og $u$ og $v$ er funksjoner av $x$
- $(u(x)+v(x))'=u'(x)+v'(x)$
- $(x^n)'=nx^{n-1}$
  id:: 68e3823d-e498-4632-8668-f6ab1e795faf
- $(k\cdot u(x))'=k\cdot u'(x)$
- $(a)'=0$
- $(\frac{1}{x})'=-\frac{1}{x^2}$
	- Kommer fra ((68e3823d-e498-4632-8668-f6ab1e795faf)) der $n=-1$
- $(\sqrt{x})'=\frac{1}{2\sqrt{x}}$
	- Kommer fra((68e3823d-e498-4632-8668-f6ab1e795faf)) der $n=\frac{1}{2}$
- $(u\cdot v)'=u'\cdot v + u \cdot v'$
- $(\frac{u}{v})'=\frac{u'\cdot v - u \cdot v'}{v^2}$
-
-